Finish variable semantics
Simplified things by just separating out the types of variables from the
type of indices; this solves the problem of checking equality of
variables (which are actually just codes, the type index isn't
important). The type mapping is static and the mapping itself is
complete, unlike for other data types, so no checks are needed in the
semantics. The only inconvenience of this approach is that the GADT
defined variables alongside their types, whereas here the definitions
are separate.

In Haskell we'll just have to unsafeCoerce, but the GADT approach
would've had the same problem since Var would have lost its nice type
indices in the extraction process.

src/Database/DataStructures.v
@@ -48,20 +48,24 @@ Axiom array_eqdec : EqualDec Array_.
 Existing Instance array_eqdec.
 Definition Array (T:ty) := Array_.
 
-(* TODO: fix Vars to be same as IORef *)
-Inductive LogVar : Type -> Type :=
-| File : LogVar Fd
-.
+Module Var.
+  Inductive t :=
+  | LogFile
+  .
 
-Inductive Var : Type -> Type :=
-| Log : forall T, LogVar T -> Var T
-.
+  Definition ty (x:t) : Type :=
+    match x with
+    | LogFile => Fd
+    end.
+End Var.
+
+Instance var_eqdec : EqualDec Var.t := _.
 
 Module Data.
   Inductive Op : Type -> Type :=
   (* generic variable operations *)
-  | GetVar : forall T, Var T -> Op T
-  | SetVar : forall T, Var T -> T -> Op T
+  | GetVar : forall (v:Var.t), Op (Var.ty v)
+  | SetVar : forall (v:Var.t), Var.ty v -> Op unit
 
   (* arbitrary references *)
   | NewIORef : forall (T:ty), T -> Op (IORef T)
@@ -77,10 +81,10 @@ Module Data.
   (* TODO: hashtables *)
   .
 
-  Definition get Op' {i:Injectable Op Op'} T (var: Var T) : proc Op' T :=
+  Definition get Op' {i:Injectable Op Op'} (var: Var.t) : proc Op' (Var.ty var) :=
     Call (inject (GetVar var)).
 
-  Definition set_var Op' {i:Injectable Op Op'} T (var: Var T) (v: T) : proc Op' T :=
+  Definition set_var Op' {i:Injectable Op Op'} (var: Var.t) (v: Var.ty var) : proc Op' unit :=
     Call (inject (SetVar var v)).
 
   Definition newIORef Op' {i:Injectable Op Op'}
@@ -106,13 +110,21 @@ Module Data.
     Call (inject (ArrayAppend a v)).
 
   Record State : Type :=
-    mkState { iorefs: IORef_ -> option {T:ty & T};
+    mkState { vars: forall (var:Var.t), Var.ty var;
+              iorefs: IORef_ -> option {T:ty & T};
               arrays: Array_ -> option {T:ty & list T};
               (* TODO: similar model for variables (except complete map) and
               arrays *) }.
 
   Instance _eta : Settable _ :=
-    mkSettable (constructor mkState <*> iorefs <*> arrays)%set.
+    mkSettable (constructor mkState <*> vars <*> iorefs <*> arrays)%set.
+
+  Definition upd_vars (var: Var.t) (v: Var.ty var) (vars: forall var, Var.ty var) :
+    forall var, Var.ty var :=
+    fun var' => match equal var var' with
+             | left H => rew [Var.ty] H in v
+             | right _ => vars var'
+             end.
 
   Definition upd_iorefs T (v: IORef T) (x: T)
              (f:IORef_ -> option {T:ty & T}) : IORef_ -> option {T:ty & T}
@@ -146,17 +158,10 @@ Module Data.
 
   Import RelationNotations.
 
-  Definition checkTy (T:ty) {F: ty -> Type} {A} (xbundle: {T:ty & F T}) : relation A A (F T) :=
-    let 'existT T0 x := xbundle in
-    match equal T0 T with
-    | left H => pure (rew [F] H in x)
-    | right _ => error
-    end.
-
   Definition step T (op:Op T) : relation State State T :=
     match op in Op T return relation State State T with
-    (* | GetVar v => reads (fun s => vars s v) *)
-    (* | SetVar v x => puts (set vars (fupd v x)) *)
+    | GetVar v => reads (fun s => vars s v)
+    | SetVar v x => puts (set vars (upd_vars v x))
     | NewIORef _ x =>
       r <- such_that (fun s r => s.(iorefs) r = None);
         _ <- puts (set iorefs (upd_iorefs r x));
@@ -179,7 +184,6 @@ Module Data.
     | ArrayGet v i =>
       l0 <- readSome (fun s => get_array v s.(arrays));
         readSome (fun _ => List.nth_error l0 (N.to_nat (uint64.(toNum) i)))
-    | _ => error
     end.
 
 End Data.
